progress havoc inhale proof (exhale cases are remaining)

TotalSemantics.thy
@@ -1,5 +1,5 @@
 theory TotalSemantics
-imports Viper.ViperLang TotalExpressions
+imports Viper.ViperLang TotalExpressions "HOL-Eisbach.Eisbach" "HOL-Eisbach.Eisbach_Tools"
 begin
 
 (*datatype 'a result = Failure | Set (select_set: "'a full_total_state set")*)
@@ -8,6 +8,18 @@ datatype 'a standard_result = RMagic | RFailure | RNormal "'a full_total_state"
 
 fun update_store_total :: "'a full_total_state \<Rightarrow> var \<Rightarrow> 'a val \<Rightarrow> 'a full_total_state"
   where "update_store_total \<omega> x v = ((get_store_total \<omega>)(x \<mapsto> v), get_trace_total \<omega>, get_hm_total_full \<omega>)"
+
+lemma update_store_total_trace_same: "get_trace_total (update_store_total \<omega> x v) = get_trace_total \<omega>"
+  by simp
+
+lemma update_store_total_hm_same: "get_hm_total_full (update_store_total \<omega> x v) = get_hm_total_full \<omega>"
+  by simp
+
+lemma update_store_total_heap_same: "get_heap_total_full (update_store_total \<omega> x v) = get_heap_total_full \<omega>"
+  by simp
+
+lemma update_store_total_mask_same: "get_mask_total_full (update_store_total \<omega> x v) = get_mask_total_full \<omega>"
+  by simp
 
 definition update_heap_total :: "'a total_state \<Rightarrow> heap_loc \<Rightarrow> 'a val \<Rightarrow> 'a total_state"
   where "update_heap_total mh l v = Abs_total_state ((get_mask_total mh), (get_heap_total mh)(l := v))"
@@ -35,11 +47,45 @@ lemma update_mask_total_multiple:
   using assms
   by (simp add: Abs_total_state_inverse_2)
 
+lemma update_heap_total_mask_same: "get_mask_total (update_heap_total \<phi> l v) = get_mask_total \<phi>"
+  unfolding update_heap_total_def
+  by (metis Abs_total_state_inverse_2 fst_conv get_mask_total.simps get_mask_total_wf wf_pre_total_state.simps)
+
+lemma Rep_total_state_inj: "Rep_total_state a = Rep_total_state b \<Longrightarrow> a = b"
+  by (metis Rep_total_state_inverse)
+
+lemma update_heap_total_overwrite: "update_heap_total (update_heap_total mh l v1) l v2 = update_heap_total mh l v2"
+  apply (rule total_state_eq)
+   apply (simp only: update_heap_total_mask_same)
+  by (metis Abs_total_state_inverse_2 fun_upd_upd get_heap_total.simps get_mask_total_wf snd_conv update_heap_total_def wf_pre_total_state.simps)
+
+lemma update_heap_total_lookup_1: "get_heap_total (update_heap_total \<phi> l v) l = v"
+  by (metis (no_types, lifting) Abs_total_state_inverse_2 fun_upd_eqD fun_upd_triv get_heap_total.simps get_mask_total_wf snd_conv update_heap_total_def wf_pre_total_state.simps)
+
+lemma update_heap_total_lookup_2: "l1 \<noteq> l2 \<Longrightarrow> get_heap_total (update_heap_total \<phi> l1 v) l2 = get_heap_total \<phi> l2"
+  by (metis (no_types, lifting) Abs_total_state_inverse_2 fun_upd_idem_iff fun_upd_triv fun_upd_twist get_heap_total.elims get_mask_total_wf sndI update_heap_total_def wf_pre_total_state.simps)
+
 fun update_heap_total_full :: "'a full_total_state \<Rightarrow> heap_loc \<Rightarrow> 'a val \<Rightarrow> 'a full_total_state"
   where "update_heap_total_full \<omega> l v = (get_store_total \<omega>, get_trace_total \<omega>, update_heap_total (get_hm_total_full \<omega>) l v )"
 
+lemma update_heap_total_full_lookup_1: "get_heap_total_full (update_heap_total_full \<phi> l v) l = v"
+  by (metis get_heap_total_full.simps get_hm_total_full.simps snd_conv update_heap_total_full.simps update_heap_total_lookup_1)
+
+lemma update_heap_total_full_lookup_2: "l1 \<noteq> l2 \<Longrightarrow> get_heap_total_full (update_heap_total_full \<phi> l1 v) l2 = get_heap_total_full \<phi> l2"
+  by (metis get_heap_total_full.simps get_hm_total_full.simps snd_conv update_heap_total_full.simps update_heap_total_lookup_2)
+
+lemma update_heap_total_overwrite_full: "update_heap_total_full (update_heap_total_full \<omega> l v1) l v2 = update_heap_total_full \<omega> l v2"
+  apply (rule full_total_state_eq)
+     apply simp
+    apply simp
+   apply (simp add: update_heap_total_overwrite)
+  by (metis get_hm_total_full.elims get_mask_total_full.elims snd_conv update_heap_total_full.simps update_heap_total_mask_same)
+  
 fun update_mask_total_full :: "'a full_total_state \<Rightarrow> mask \<Rightarrow> 'a full_total_state"
   where "update_mask_total_full \<omega> m = (get_store_total \<omega>, get_trace_total \<omega>, update_mask_total (get_hm_total_full \<omega>) m)"
+
+lemma update_heap_total_full_mask_same: "get_mask_total_full (update_heap_total_full \<omega> l v) = get_mask_total_full \<omega>"
+  by (metis get_hm_total_full.simps get_mask_total_full.simps snd_conv update_heap_total_full.simps update_heap_total_mask_same)
 
 lemma get_update_mask_total_full: 
   assumes "wf_mask_simple m0"
@@ -103,8 +149,6 @@ definition singleton_total_wildcard :: "bool \<Rightarrow> heap_loc \<Rightarrow
   where "singleton_total_wildcard havoc_new l v \<sigma> \<tau> =
            { \<omega> | \<omega> p. p \<noteq> pnone \<and> get_store_total \<omega> = \<sigma> \<and> get_trace_total \<omega> = \<tau> \<and> 
                     get_mask_total_full \<omega> = (zero_mask(l := p)) \<and> (\<not>havoc_new \<longrightarrow> get_heap_total_full \<omega> l = v)}"
-
-term update_mask_total_full
 
 (*
 
@@ -476,17 +520,26 @@ inductive red_stmt_total_single_set :: "program \<Rightarrow> 'a interp \<Righta
    "\<lbrakk> wd_pure_exp_total Pr \<Delta> CInhale e_r \<omega>; 
       wd_pure_exp_total Pr \<Delta> CInhale e \<omega>; 
       Pr, \<Delta> \<turnstile> \<langle>e_r; \<omega>\<rangle> [\<Down>]\<^sub>t Val (VRef (Address addr));
+      get_mask_total_full \<omega> (addr,f) \<noteq> pnone;
       Pr, \<Delta>  \<turnstile> \<langle>e; \<omega>\<rangle> [\<Down>]\<^sub>t Val v \<rbrakk> \<Longrightarrow> 
       red_stmt_total_single_set Pr \<Delta> conf (FieldAssign e_r f e) \<omega> (Inr (), (RNormal (update_heap_total_full \<omega> (addr,f) v)))"
  | RedFieldAssignFailure: 
-   "\<lbrakk> \<not> wd_pure_exp_total Pr \<Delta> CInhale e_r \<omega> \<or> \<not> wd_pure_exp_total Pr \<Delta> CInhale e \<omega> \<or> (Pr, \<Delta> \<turnstile> \<langle>e_r; \<omega>\<rangle> [\<Down>]\<^sub>t Val (VRef Null)) \<rbrakk> \<Longrightarrow> 
+   "\<lbrakk> \<not> wd_pure_exp_total Pr \<Delta> CInhale e_r \<omega> \<or> 
+      \<not> wd_pure_exp_total Pr \<Delta> CInhale e \<omega> \<or> 
+      (Pr, \<Delta> \<turnstile> \<langle>e_r; \<omega>\<rangle> [\<Down>]\<^sub>t Val (VRef Null)) \<or> 
+      get_mask_total_full \<omega> (addr,f) \<noteq> pnone \<rbrakk> \<Longrightarrow> 
       red_stmt_total_single_set Pr \<Delta> conf (FieldAssign e_r f e) \<omega> (Inr (), RFailure)"
  | RedIfTrue: 
-   "\<lbrakk> Pr,\<Delta> \<turnstile> \<langle>e_b; \<omega>\<rangle> [\<Down>]\<^sub>t Val (VBool True) \<rbrakk> \<Longrightarrow> 
+   "\<lbrakk> Pr,\<Delta> \<turnstile> \<langle>e_b; \<omega>\<rangle> [\<Down>]\<^sub>t Val (VBool True);
+     wd_pure_exp_total Pr \<Delta> CInhale e_b \<omega> \<rbrakk> \<Longrightarrow> 
       red_stmt_total_single_set Pr \<Delta> conf (If e_b s1 s2) \<omega> (Inl s1, RNormal \<omega>)"
  | RedIfFalse: 
-   "\<lbrakk> Pr,\<Delta> \<turnstile> \<langle>e_b; \<omega>\<rangle> [\<Down>]\<^sub>t Val (VBool False) \<rbrakk> \<Longrightarrow> 
+   "\<lbrakk> Pr,\<Delta> \<turnstile> \<langle>e_b; \<omega>\<rangle> [\<Down>]\<^sub>t Val (VBool False);
+      wd_pure_exp_total Pr \<Delta> CInhale e_b \<omega> \<rbrakk> \<Longrightarrow> 
       red_stmt_total_single_set Pr \<Delta> conf (If e_b s1 s2) \<omega> (Inl s2, RNormal \<omega>)"
+ | RedIfFailure:
+    "\<lbrakk> \<not>wd_pure_exp_total Pr \<Delta> CInhale e_b \<omega> \<rbrakk> \<Longrightarrow>
+       red_stmt_total_single_set Pr \<Delta> conf (If e_b s1 s2) \<omega> (Inr (), RFailure)"
  | RedSeq1:
    "\<lbrakk> red_stmt_total_single_set Pr \<Delta> conf s1 \<omega> (Inl s'', r'') \<rbrakk> \<Longrightarrow>
       red_stmt_total_single_set Pr \<Delta> conf (Seq s1 s2) \<omega> (Inl (Seq s'' s2), r'')"
@@ -544,11 +597,25 @@ subsection \<open>Backwards simulation\<close>
 
 definition lift_sim_rel :: "'a simulation_rel \<Rightarrow> 'a stmt_config \<Rightarrow> 'a stmt_config \<Rightarrow> bool"
   where "lift_sim_rel R w1 w2 \<equiv>
-            (is_failure_config w1 \<and> is_failure_config w2) \<or>
+            (is_failure_config w1 \<and> is_failure_config w2 \<and> fst w1 = fst w2) \<or>
             (\<exists>\<omega>1 \<omega>2. is_normal_config w1 \<omega>1 \<and> is_normal_config w2 \<omega>2 \<and> R \<omega>1 \<omega>2 \<and> fst w1 = fst w2)"
 
 lemma lift_sim_rel_fail: "lift_sim_rel R w1 w2 \<Longrightarrow> is_failure_config w1 \<Longrightarrow> is_failure_config w2"
   by (simp add: lift_sim_rel_def)
+
+lemma lift_sim_rel_fail_2: "lift_sim_rel R w1 w2 \<Longrightarrow> is_failure_config w1 \<Longrightarrow> fst w1 = fst w2 \<and> snd w2 = RFailure"
+  by (simp add: lift_sim_rel_def)
+
+lemma lift_sim_rel_fail_3: "lift_sim_rel R w1 w2 \<Longrightarrow> w1 = (Inr (), RFailure) \<Longrightarrow> w2 = (Inr (), RFailure)"
+  unfolding lift_sim_rel_def
+  by (metis is_failure_config.elims(2) is_failure_config.elims(3) lift_sim_rel_def lift_sim_rel_fail prod.exhaust_sel snd_conv)
+
+lemma lift_sim_rel_normal: "lift_sim_rel R w1 w2 \<Longrightarrow> is_normal_config w1 \<omega>1 \<Longrightarrow> 
+                              fst w1 = fst w2 \<and> (\<exists>\<omega>2. is_normal_config w2 \<omega>2 \<and> R \<omega>1 \<omega>2)"
+  unfolding lift_sim_rel_def by auto
+
+lemma lift_sim_rel_not_magic: "lift_sim_rel R w1 w2 \<Longrightarrow> snd w1 \<noteq> RMagic \<and> snd w2 \<noteq> RMagic"
+  unfolding lift_sim_rel_def by fastforce
 
 lemma red_stmt_total_start_normal:
   assumes "red_stmt_total_single Pr \<Delta> conf w1 w2"
@@ -592,8 +659,7 @@ qed
 
 lemma result_normal_exhaust: 
    "w \<noteq> RMagic \<Longrightarrow> w \<noteq> RFailure \<Longrightarrow> \<exists>\<omega>. w = RNormal \<omega>"
-  apply (cases w)
-  by auto
+  by (cases w) auto
 
 lemma stmt_config_normal_exhaust:
   assumes "\<not>is_failure_config w" and "snd w \<noteq> RMagic"
@@ -606,7 +672,7 @@ proof -
     by simp
 qed
 
-lemma lift_total_rel: 
+lemma lift_total_rel:
   assumes "\<forall>\<omega>. \<exists> \<omega>'. R \<omega> \<omega>'"
   shows "\<forall>w :: 'a stmt_config. snd w \<noteq> RMagic \<longrightarrow> (\<exists>w'. lift_sim_rel R w w')"
 proof (rule allI, rule impI)+
@@ -653,8 +719,6 @@ proof ( (rule allI | rule impI) +)
   qed (simp)
 qed
 
-
-
 definition havoc_rel :: "'a simulation_rel"
   where "havoc_rel \<omega> \<omega>' \<equiv> get_mask_total_full \<omega> = get_mask_total_full \<omega>' \<and> 
                           equal_on_mask (get_mask_total_full \<omega>) (get_heap_total_full \<omega>) (get_heap_total_full \<omega>') \<and>
@@ -672,9 +736,8 @@ lemma havoc_rel_same_store: "havoc_rel \<omega> \<omega>' \<Longrightarrow> get_
 lemma havoc_rel_same_mask: "havoc_rel \<omega> \<omega>' \<Longrightarrow> get_mask_total_full \<omega> = get_mask_total_full \<omega>'"
   by (simp add: havoc_rel_def)
 
-lemma havoc_rel_heap_equal_on_mask: "havoc_rel \<omega> \<omega>' \<Longrightarrow> equal_on_mask (get_mask_total_full \<omega>) (get_heap_total_full \<omega>) (get_heap_total_full \<omega>')"
-  unfolding havoc_rel_def
-  oops 
+lemma havoc_rel_refl: "havoc_rel \<omega> \<omega>"
+  by (simp add: equal_on_mask_refl havoc_rel_def)
 
 lemma havoc_rel_sym: "havoc_rel \<omega> \<omega>' \<Longrightarrow> havoc_rel \<omega>' \<omega>"
   by (simp add: havoc_rel_def equal_on_mask_def)
@@ -825,8 +888,8 @@ proof -
     done
 qed
 
-lemma havoc_inhale_rel:
-  assumes "red_inhale Pr \<Delta> True inh_assume A \<omega> res" and "res = RNormal \<omega>'" and "havoc_rel \<omega>' \<omega>2'" (*and "supported_subset A"*)
+lemma havoc_inhale_normal_rel:
+  assumes "red_inhale Pr \<Delta> True inh_assume A \<omega> res" and "res = RNormal \<omega>'" and "havoc_rel \<omega>' \<omega>2'" 
   shows "red_inhale Pr \<Delta> False inh_assume A (update_mask_total_full \<omega>2' (get_mask_total_full \<omega>)) (RNormal \<omega>2') \<and> havoc_rel \<omega> (update_mask_total_full \<omega>2' (get_mask_total_full \<omega>))"
   using assms
 proof (induction arbitrary: \<omega>' \<omega>2')
@@ -1011,66 +1074,302 @@ next
     done
 qed (auto)
 
-lemma step_havoc_rel:
-  assumes "red_stmt_total_single Pr \<Delta> \<lparr>havoc_inhale=True\<rparr> (Inl s,  RNormal \<omega>) w'"
-  shows   "(is_failure_config w' \<longrightarrow> (\<exists>\<omega>2 w2'. havoc_rel \<omega> \<omega>2 \<and> red_stmt_total_single Pr \<Delta> \<lparr>havoc_inhale=False\<rparr> (Inl s, RNormal \<omega>2) w2' \<and> is_failure_config w2')) \<and>
-                (\<forall> s' \<omega>' \<omega>2'. is_normal_config w' \<omega>' \<longrightarrow> havoc_rel \<omega>' \<omega>2' \<longrightarrow>
-                               (\<exists>\<omega>2. havoc_rel \<omega> \<omega>2 \<and> red_stmt_total_single Pr \<Delta> \<lparr>havoc_inhale=False\<rparr> (Inl s, RNormal \<omega>2) (Inl s', RNormal \<omega>2')))"
+method inh_fail_basic_tac for \<omega> :: "'a full_total_state" uses local_assms intro = 
+  (rule exI[where ?x=\<omega>], 
+   rule conjI[OF havoc_rel_refl],
+   insert local_assms,
+   blast intro!:intro)
+
+lemma havoc_inhale_failure_rel:
+  assumes "red_inhale Pr \<Delta> True inh_assume A \<omega> res" and "res = RFailure"
+  shows "\<exists> \<omega>2. havoc_rel \<omega> \<omega>2 \<and> red_inhale Pr \<Delta> False inh_assume A \<omega>2 RFailure"
   using assms
-  proof (cases)
-    case NormalSingleStep
-    then show ?thesis
-      sorry
+proof (induction)
+  case (InhSepNormal inh_assume A \<omega> \<omega>A B res)
+  from this obtain \<omega>B where
+     "havoc_rel \<omega>A \<omega>B" and "red_inhale Pr \<Delta> False inh_assume B \<omega>B RFailure"
+    by auto
+  thus ?case
+    using havoc_inhale_normal_rel InhSepNormal.hyps(1) red_inhale.InhSepNormal by blast
+next
+  case (InhSepFailureMagic inh_assume A \<omega> resA B)
+  then show ?case 
+    using red_inhale.InhSepFailureMagic by blast
+next
+  case (InhImpTrue e \<omega> inh_assume A res)
+  then show ?case 
+    by (meson InhImpFailure havoc_rel_expr_eval_same red_inhale.InhImpTrue)
+next
+  case (InhImpFailure e \<omega> inh_assume A)
+  then show ?case 
+  by (meson havoc_rel_sym havoc_rel_wd_same red_inhale.InhImpFailure total_havoc_rel)
+next
+  case (AssumeAcc e_r \<omega> a e_p p f)
+  then show ?case by (simp split: if_split_asm)
+next
+case (InhAssumeAccFail2 e_r \<omega> a e_p p inh_assume f)
+  show ?case 
+    by (inh_fail_basic_tac \<omega> local_assms:local.InhAssumeAccFail2 intro: red_inhale.InhAssumeAccFail2)
+next
+case (AssumeAccWildcard e_r \<omega> a f)
+  then show ?case by (simp split: if_split_asm)
+next
+  case (InhAssumeAccWildcardFail2 e_r \<omega> a e_p p inh_assume f)
+    show ?case 
+     by (inh_fail_basic_tac \<omega> local_assms:local.InhAssumeAccWildcardFail2 intro: red_inhale.InhAssumeAccWildcardFail2)   
+next
+  case (InhInhaleExhale inh_assume A \<omega> res B)
+  then show ?case
+  using red_inhale.InhInhaleExhale by blast
+next
+  case (InhPureNormalMagic e \<omega> b inh_assume)
+  then show ?case by (simp split: if_split_asm)
+next
+  case (InhPureFail e \<omega> inh_assume)
+  show ?case 
+    by (inh_fail_basic_tac \<omega> local_assms:local.InhPureFail intro: red_inhale.InhPureFail)
+qed auto
+
+lemma havoc_rel_store_update:
+  assumes "havoc_rel (update_store_total \<omega> x v) \<omega>1"
+  shows "\<exists>\<omega>2. \<omega>1 = update_store_total \<omega>2 x v"
+  using assms
+  unfolding havoc_rel_def
+  by (metis Rep_total_state_inverse fstI fun_upd_same fun_upd_triv get_heap_total_full.simps get_hm_total_full_comp update_mask_total_def update_mask_total_full.simps update_mask_total_full_same update_store_total.elims)
+
+lemma havoc_rel_store_update_3:
+  assumes "havoc_rel (update_store_total \<omega> x v) \<omega>2'"
+  shows "\<exists>\<omega>2. \<omega>2' = update_store_total \<omega>2 x v \<and> havoc_rel \<omega> \<omega>2"
+proof -
+  from assms obtain \<omega>2_first where "\<omega>2' = update_store_total \<omega>2_first x v" 
+    using havoc_rel_store_update by blast
+  hence *:"get_mask_total_full \<omega>2' = get_mask_total_full \<omega>2_first"
+    by (simp add: update_store_total_mask_same)
+  have **:"equal_on_mask (get_mask_total_full \<omega>) (get_heap_total_full \<omega>) (get_heap_total_full \<omega>2_first)"
+    using assms \<open>\<omega>2' = _\<close> update_store_total_heap_same update_store_total_mask_same
+    unfolding havoc_rel_def
+    by fastforce
+ 
+  let ?\<omega>2 = "(get_store_total \<omega>, get_trace_total \<omega>2_first, get_hm_total_full \<omega>2_first)"
+  have "havoc_rel \<omega> ?\<omega>2"
+    unfolding havoc_rel_def
+    apply (intro conjI)
+       using * assms havoc_rel_same_mask apply fastforce
+     using ** apply simp
+    apply simp
+    done
+
+  show ?thesis
+    apply (rule exI[where ?x="?\<omega>2"])
+    apply (rule conjI)
+     apply (rule full_total_state_eq)
+        using \<open>\<omega>2' = _\<close>
+        apply (metis Pair_inject assms havoc_rel_same_store update_mask_total_full.simps update_mask_total_full_same update_store_total.simps)
+       apply (simp add: \<open>\<omega>2' = _\<close>)
+      apply (simp add: \<open>\<omega>2' = _\<close>)
+     apply (metis \<open>havoc_rel \<omega> _\<close> assms havoc_rel_same_mask update_store_total_mask_same)
+    using \<open>havoc_rel \<omega> _\<close> by auto
+qed
+
+lemma havoc_rel_heap_update:
+  assumes "havoc_rel (update_heap_total_full \<omega> l v) \<omega>2'" and "get_mask_total_full \<omega> l \<noteq> pnone"
+  shows "\<exists>\<omega>2. \<omega>2' = (update_heap_total_full \<omega>2 l v) \<and> havoc_rel \<omega> \<omega>2"
+proof -
+  let ?h ="get_heap_total_full \<omega>"
+  let ?\<omega>2="update_heap_total_full \<omega>2' l (?h l)"
+
+  from assms have HeapLoc:"get_heap_total_full \<omega>2' l = v"
+    apply (unfold havoc_rel_def)
+    apply (unfold equal_on_mask_def)
+    by (metis update_heap_total_full_lookup_1 update_heap_total_full_mask_same)
+
+  show ?thesis
+    apply (rule exI[where ?x="?\<omega>2"])
+    apply (rule conjI)
+     apply (rule full_total_state_eq)
+        apply simp
+       apply simp
+      apply (simp only: update_heap_total_overwrite_full)
+      apply (rule HOL.ext)
+      apply (case_tac "x = l")
+       apply (simp only: update_heap_total_full_lookup_1)
+       apply (rule HeapLoc)
+      apply (rule HOL.sym[OF update_heap_total_full_lookup_2])
+      apply simp
+     apply (simp only: update_heap_total_full_mask_same)
+    unfolding havoc_rel_def
+    apply (intro conjI)
+     apply (simp only: update_heap_total_full_mask_same)
+      apply (metis assms(1) havoc_rel_same_mask update_heap_total_full_mask_same)
+    apply (smt (z3) assms equal_on_mask_def havoc_rel_def update_heap_total_full_lookup_1 update_heap_total_full_lookup_2 update_heap_total_full_mask_same)
+    by (metis assms(1) fstI get_store_total.simps havoc_rel_same_store update_heap_total_full.simps)
 qed
 
 
-lemma havoc_conf_equiv:
-  assumes "stmt_verifies_total dummy Pr \<lparr>havoc_inhale=False\<rparr> s"
-  shows "stmt_verifies_total dummy Pr \<lparr>havoc_inhale=True\<rparr> s"
-proof (rule backwards_simulation)
+lemma step_havoc_rel:
+  assumes "red_stmt_total_single Pr \<Delta> \<lparr>havoc_inhale=True\<rparr> (Inl s,  RNormal \<omega>) w'" and 
+          "lift_sim_rel havoc_rel w' w2'"
+  (*shows   "(is_failure_config w' \<longrightarrow> (\<exists>\<omega>2 w2'. havoc_rel \<omega> \<omega>2 \<and> red_stmt_total_single Pr \<Delta> m\<lparr>havoc_inhale=False\<rparr> (Inl s, RNormal \<omega>2) w2' \<and> is_failure_config w2')) \<and>
+                (\<forall> s' \<omega>' \<omega>2'. is_normal_config w' \<omega>' \<longrightarrow> havoc_rel \<omega>' \<omega>2' \<longrightarrow>
+                               (\<exists>\<omega>2. havoc_rel \<omega> \<omega>2 \<and> red_stmt_total_single Pr \<Delta> \<lparr>havoc_inhale=False\<rparr> (Inl s, RNormal \<omega>2) (Inl s', RNormal \<omega>2')))"*)
+  shows "\<exists>\<omega>2. havoc_rel \<omega> \<omega>2 \<and> red_stmt_total_single Pr \<Delta> \<lparr>havoc_inhale=False\<rparr> (Inl s, RNormal \<omega>2) w2'"
+  using assms
+  proof (cases)
+    case NormalSingleStep
+    then show ?thesis using assms(2)
+    proof (induction arbitrary: w2')
+      case RedSkip
+      then show ?case
+       by (metis (no_types, lifting) assms(2) fst_conv is_failure_config.simps is_normal_config.elims(2) lift_sim_rel_def prod.exhaust_sel red_stmt_total_single.NormalSingleStep red_stmt_total_single_set.RedSkip snd_conv standard_result.distinct(5) standard_result.inject)
+    next
+    case (RedInhale A \<omega> res)
+    show ?case
+    proof (cases res)
+    case RMagic
+    then show ?thesis 
+      using assms(2) lift_sim_rel_not_magic
+      by (metis RedInhale.prems snd_conv)
+    next
+      case RFailure
+      with RedInhale have "w2' = (Inr (), RFailure)"
+        unfolding lift_sim_rel_def
+        using RedInhale.prems lift_sim_rel_fail_3 by blast
+      with RFailure RedInhale NormalSingleStep assms(2) havoc_inhale_failure_rel
+      show ?thesis
+        by (metis conf.select_convs(1) red_stmt_total_single.NormalSingleStep red_stmt_total_single_set.RedInhale)
+    next
+      case (RNormal \<omega>')
+      with RedInhale obtain \<omega>2' where "w2' = (Inr (), RNormal \<omega>2')" and "havoc_rel \<omega>' \<omega>2'"
+        unfolding lift_sim_rel_def      
+        by (metis fst_conv is_failure_config.simps is_normal_config.elims(2) snd_conv standard_result.distinct(5) standard_result.inject surjective_pairing)
+      with \<open>res = _\<close> RedInhale assms(2) havoc_inhale_normal_rel
+      obtain \<omega>2 where "havoc_rel \<omega> \<omega>2" and "red_inhale Pr \<Delta> False False A \<omega>2 (RNormal \<omega>2')"
+        by (metis (full_types) conf.select_convs(1))
+      then show ?thesis
+        by (metis \<open>w2' = (Inr (), RNormal \<omega>2')\<close> conf.select_convs(1) local.RedInhale(1) red_stmt_total_single.NormalSingleStep red_stmt_total_single_set.RedInhale)
+    qed
+    next
+      case (RedExhale A m' \<omega>')
+      then show ?case sorry
+    next
+      case (RedExhaleFailure A)
+      then show ?case sorry
+    next
+      case (RedAssert A m')
+      then show ?case sorry
+    next
+      case (RedAssertFailure A)
+      then show ?case sorry
+    next
+      case (RedLocalAssign e \<omega> v x)
+      from assms(2) obtain \<omega>2' \<omega>2 where "w2' = (Inr (), RNormal \<omega>2')" and 
+        "\<omega>2' = update_store_total \<omega>2 x v" and HRel:"havoc_rel \<omega> \<omega>2"
+        using havoc_rel_store_update_3
+        unfolding lift_sim_rel_def      
+        by (metis RedLocalAssign.prems fst_conv is_normal_config.simps lift_sim_rel_normal snd_conv surjective_pairing)
+      show ?case
+        apply (rule exI)
+        apply (rule conjI[OF HRel])
+        apply (subst \<open>w2' = _\<close>, subst \<open>\<omega>2' = _\<close>)
+        apply (rule, rule)
+         apply (rule havoc_rel_wd_same[OF \<open>wd_pure_exp_total _ _ _ e \<omega>\<close> HRel])
+        apply (rule havoc_rel_expr_eval_same[OF \<open>_, _ \<turnstile> \<langle>e;\<omega>\<rangle> [\<Down>]\<^sub>t _\<close> \<open>wd_pure_exp_total _ _ _ e \<omega>\<close> HRel])
+        done
+    next
+      case (RedLocalAssignFailure e \<omega> x)
+      have "w2' = (Inr (), RFailure)" 
+        using RedLocalAssignFailure.prems lift_sim_rel_fail_3 by blast
+      show ?case
+        apply (rule exI[where ?x = \<omega>])
+        apply (rule conjI[OF havoc_rel_refl])
+        apply (subst \<open>w2' = _\<close>)
+        apply (rule, rule)
+        by (rule \<open>\<not>_\<close>)
+    next
+      case (RedFieldAssign e_r \<omega> e addr f v)
+      from assms(2) havoc_rel_heap_update \<open>get_mask_total_full \<omega> (addr, f) \<noteq> pnone\<close> obtain \<omega>2 where
+        HRel:"havoc_rel \<omega> \<omega>2" and "w2' = (Inr (), RNormal (update_heap_total_full \<omega>2 (addr, f) v))"
+        unfolding lift_sim_rel_def
+        by (metis RedFieldAssign.prems fst_conv is_normal_config.simps lift_sim_rel_normal snd_conv surjective_pairing)
+      show ?case
+        apply (rule exI)
+        apply (rule conjI[OF HRel])
+        apply (subst \<open>w2' = _\<close>)
+        apply (rule, rule)
+            apply (rule havoc_rel_wd_same[OF \<open>wd_pure_exp_total _ _ _ e_r \<omega>\<close> HRel])
+          apply (rule havoc_rel_wd_same[OF \<open>wd_pure_exp_total _ _ _ e \<omega>\<close> HRel])
+          apply (rule havoc_rel_expr_eval_same[OF \<open>_, _ \<turnstile> \<langle>e_r;\<omega>\<rangle> [\<Down>]\<^sub>t _\<close> \<open>wd_pure_exp_total _ _ _ e_r \<omega>\<close> HRel])
+         apply (metis \<open>get_mask_total_full \<omega> (addr, f) \<noteq> pnone\<close> HRel havoc_rel_same_mask)
+        apply (rule havoc_rel_expr_eval_same[OF \<open>_, _ \<turnstile> \<langle>e;\<omega>\<rangle> [\<Down>]\<^sub>t _\<close> \<open>wd_pure_exp_total _ _ _ e \<omega>\<close> HRel])
+        done
+    next
+      case (RedFieldAssignFailure e_r \<omega> e f)
+      hence "w2' = (Inr (), RFailure)"
+        using lift_sim_rel_fail_3 by blast       
+      show ?case
+        apply (rule exI)
+        apply (rule conjI[OF havoc_rel_refl])
+        apply (subst \<open>w2' = _\<close>)
+        apply (rule, rule) 
+        apply (rule RedFieldAssignFailure(1))
+        done    
+    next
+      case (RedIfTrue e_b \<omega> s1 s2)
+      from this obtain \<omega>2 where HRel:"havoc_rel \<omega> \<omega>2" and "w2' = (Inl s1, RNormal \<omega>2)"      
+        by (metis (no_types, lifting) assms(2) fst_conv is_failure_config.simps is_normal_config.simps lift_sim_rel_def prod.exhaust_sel snd_conv standard_result.distinct(5) standard_result.inject)
+      show ?case 
+        apply (rule exI)
+        apply (rule conjI[OF HRel])
+        apply (subst \<open>w2' = _\<close>)
+        apply (rule, rule)
+         apply (rule havoc_rel_expr_eval_same[OF \<open>_, _ \<turnstile> \<langle>e_b; \<omega>\<rangle> [\<Down>]\<^sub>t _\<close> \<open>wd_pure_exp_total _ _ _ e_b \<omega>\<close> HRel])
+        apply (rule havoc_rel_wd_same[OF \<open>wd_pure_exp_total _ _ _ e_b \<omega>\<close> HRel])
+        done
+    next
+      case (RedIfFalse e_b \<omega> s1 s2)
+        from this obtain \<omega>2 where HRel:"havoc_rel \<omega> \<omega>2" and "w2' = (Inl s2, RNormal \<omega>2)"      
+        by (metis (no_types, lifting) assms(2) fst_conv is_failure_config.simps is_normal_config.simps lift_sim_rel_def prod.exhaust_sel snd_conv standard_result.distinct(5) standard_result.inject)
+      show ?case
+        apply (rule exI)
+        apply (rule conjI[OF HRel])
+        apply (subst \<open>w2' = _\<close>)
+        apply (rule, rule)
+         apply (rule havoc_rel_expr_eval_same[OF \<open>_, _ \<turnstile> \<langle>e_b; \<omega>\<rangle> [\<Down>]\<^sub>t _\<close> \<open>wd_pure_exp_total _ _ _ e_b \<omega>\<close> HRel])
+        apply (rule havoc_rel_wd_same[OF \<open>wd_pure_exp_total _ _ _ e_b \<omega>\<close> HRel])
+        done
+    next 
+      case (RedIfFailure e_b s1 s2)
+      hence "w2' = (Inr (), RFailure)"
+        using assms(2) lift_sim_rel_fail_3 by blast
+      show ?case
+        apply (rule exI)
+        apply (rule conjI[OF havoc_rel_refl])
+        apply (subst \<open>w2' = _\<close>)
+        apply (rule, rule)
+        apply (rule \<open>\<not>_\<close>)
+        done
+    next
+      case (RedSeq1 s1 \<omega> s'' r'' s2)      
+      from \<open>lift_sim_rel _ _ w2'\<close> obtain r2' where "w2' = (Inl (Seq s'' s2), r2')"
+        unfolding lift_sim_rel_def
+        by (metis eq_fst_iff)
+      from \<open>w2' = _\<close> \<open>lift_sim_rel _ _ w2'\<close> have Rel:"lift_sim_rel havoc_rel (Inl s'', r'') (Inl s'', r2')"
+        unfolding lift_sim_rel_def
+        by auto
+      from RedSeq1.IH[OF Rel] show ?case 
+        by (metis Inl_inject Pair_inject \<open>w2' = _\<close> red_stmt_total_single.NormalSingleStep red_stmt_total_single.cases red_stmt_total_single_set.RedSeq1)        
+    next
+      case (RedSeq2 s1 \<omega> r'' s2)      
+      from \<open>lift_sim_rel _ _ w2'\<close> obtain r2' where "w2' = (Inl s2, r2')"
+        unfolding lift_sim_rel_def
+        by (metis fst_conv surjective_pairing)
+      from \<open>w2' = _\<close> \<open>lift_sim_rel _ _ w2'\<close> have Rel:"lift_sim_rel havoc_rel (Inr (), r'') (Inr (), r2')"
+        unfolding lift_sim_rel_def
+        by auto
+      from RedSeq2.IH[OF Rel] show ?case
+        by (metis \<open>w2' = _\<close> prod.inject red_stmt_total_single.NormalSingleStep red_stmt_total_single.cases red_stmt_total_single_set.RedSeq2 sum.inject(1))     
+    qed
+qed
 
-
-
-
-
-(*
-inductive red_stmt_total_single_2 :: "'a program \<Rightarrow> conf \<Rightarrow> stmt \<Rightarrow> 'a stmt_config_2  \<Rightarrow> 'a stmt_config_2 \<Rightarrow> bool" where
-  "red_stmt_total_single_2 Pr conf s Normal C1 C2 =
-         (\<forall> "
-*)
-
-(*datatype 'a stmt_config_2 = SmallStepFailure | Normal "( (stmt + unit) \<times> 'a result) set"*)
-
-(*type_synonym 'a stmt_config_3 = "((stmt + unit) \<times> *)
-(*
-fun small_step_lifted :: "'a program \<Rightarrow> conf \<Rightarrow> 'a stmt_config_2 \<Rightarrow> 'a stmt_config_2 \<Rightarrow> bool"
-  where 
-    "small_step_lifted Pr conf S S' = 
-*)         
-(*
-  | "small_step_lifted Pr conf (Normal S) = 
-       (if (\<exists>s \<omega> m'. (Inl s, \<omega>) \<in> S \<and> red_stmt_total_single Pr conf s \<omega> (m', Failure)) then
-          SmallStepFailure
-       else 
-         Normal {(m', \<omega>') | s \<omega> m' \<omega>' W'. (Inl s, \<omega>) \<in> S \<and> \<omega>' \<in> W' \<and> red_stmt_total_single Pr conf s \<omega> (m', Set W')})"
-*)
-
-(*
-fun small_step_lifted :: "'a program \<Rightarrow> conf \<Rightarrow> 'a stmt_config_2 \<Rightarrow> 'a stmt_config_2"
-  where 
-    "small_step_lifted Pr conf SmallStepFailure = SmallStepFailure"
-  | "small_step_lifted Pr conf (Normal S) = 
-       (if (\<exists>s \<omega> m'. (Inl s, \<omega>) \<in> S \<and> red_stmt_total_single Pr conf s \<omega> (m', Failure)) then
-          SmallStepFailure
-       else 
-         Normal {(m', \<omega>') | s \<omega> m' \<omega>' W'. (Inl s, \<omega>) \<in> S \<and> \<omega>' \<in> W' \<and> red_stmt_total_single Pr conf s \<omega> (m', Set W')})"
-*)
-(*
-definition small_step_multi :: "'a program \<Rightarrow> conf \<Rightarrow> 'a stmt_config_2 \<Rightarrow> 'a stmt_config_2 \<Rightarrow> bool"
-  where "small_step_multi Pr conf = rtranclp (small_step_lifted Pr conf)"
-
-definition ver_total :: "'a program \<Rightarrow> conf \<Rightarrow> stmt \<Rightarrow> ('a full_total_state) set \<Rightarrow> bool" where
-  "ver Pr conf s \<omega> \<longleftrightarrow> (\<exists>r. red_stmt_total_single Pr conf s \<omega> (Set r))"
-*)
 
 end
